theories/source.v
@@ -1,63 +1,86 @@
 From stdpp Require Import binders strings gmap.
 From iris.heap_lang Require Import notation lang.
 
-Inductive aexpr :=
-  | Unit
-  | Var (x : string)
-  | Lam (x : binder) (a : aexpr)
-  | App (a1 a2 : aexpr)
-  | Pair (a1 a2 : aexpr)
-  | Split (x1 x2 : binder) (a1 a2 : aexpr)
-  | New (a : aexpr)
-  | Swap (a1 a2 : aexpr)
-.
+Section lang.
+  Inductive aexpr :=
+    | Unit
+    | Var (x : string)
+    | Lam (x : binder) (a : aexpr)
+    | App (a1 a2 : aexpr)
+    | Pair (a1 a2 : aexpr)
+    | Split (x1 x2 : binder) (a1 a2 : aexpr)
+    | New (a : aexpr)
+    | Swap (a1 a2 : aexpr)
+  .
 
-Inductive ty :=
-  | One
-  | Tensor (τ1 τ2 : ty)
-  | Fun (τ1 τ2 : ty)
-  | Unq (τ : ty)
-.
+  Inductive ty :=
+    | One
+    | Tensor (τ1 τ2 : ty)
+    | Fun (τ1 τ2 : ty)
+    | Unq (τ : ty)
+  .
+End lang.
 
-Definition ctx := gmap string ty.
+(* Mostly from DFSL paper. They store names as `binding`s
+   and use an anonymization when they cons on, but for now
+   we instead have a requirement for names being fresh *)
+Section context.
+  Inductive ctx_item := CtxItem {
+    ctx_item_name : string;
+    ctx_item_type : ty;
+  }.
 
-(* I literally just copied this from random STLC notation thing *)
-Reserved Notation "Γ ⊢ a : τ '~~>' e" (at level 74, a, τ, e at next level).
+  Definition ctx := list ctx_item.
 
-(* NOTE: I fear that overriding with ∪ for merging contexts is actually bad *)
+  Global Instance ctx_lookup : Lookup string ty ctx := 
+    fix f x Γ :=
+      match Γ with
+      | [] => None
+      | CtxItem name τ :: rest => 
+          if decide (name = x) then Some τ else f x rest
+      end.
+End context.
 
-Inductive compile : ctx → aexpr → ty → expr → Prop :=
-  | CUnit Γ :
-      Γ ⊢ Unit : One ~~> #()
-  | CVar Γ x τ :
-    Γ !! x = Some τ →
-      Γ ⊢ (Var x) : τ ~~> x
-  | CLam Γ x a τ1 τ2 e :
-    (<[ x := τ1 ]> Γ) ⊢ a : τ2 ~~> e →
-      Γ ⊢ (Lam (BNamed x) a) : (Fun τ1 τ2) ~~> λ: x, e
-  | CApp Γ1 Γ2 a1 a2 τ1 τ2 e1 e2 :
-    Γ1 ⊢ a1 : (Fun τ1 τ2) ~~> e1 →
-    Γ2 ⊢ a2 : τ1 ~~> e2 →
-      (Γ1 ∪ Γ2) ⊢ (App a1 a2) : τ2 ~~> e1 e2
-  | CPair Γ1 Γ2 a1 a2 τ1 τ2 e1 e2 :
-    Γ1 ⊢ a1 : τ1 ~~> e1 →
-    Γ2 ⊢ a2 : τ2 ~~> e2 →
-      (Γ1 ∪ Γ2) ⊢ (Pair a1 a2) : (Tensor τ1 τ2) ~~> (e1, e2)
-  | CSplit Γ1 Γ2 x1 x2 a1 a2 τ1 τ2 τ e1 e2 :
-    Γ1 ⊢ a1 : (Tensor τ1 τ2) ~~> e1 →
-    (<[ x2 := τ2 ]> (<[ x1 := τ1 ]> Γ2)) ⊢ a2 : τ ~~> e2 →
-      (Γ1 ∪ Γ2) ⊢ (Split (BNamed x1) (BNamed x2) a1 a2) : τ ~~>
-        let: "tmp" := e1 in
-        let: x1 := Fst "tmp" in
-        let: x2 := (Snd "tmp") in e2
-  | CNew Γ a τ e :
-    Γ ⊢ a : τ ~~> e →
-      Γ ⊢ (New a) : (Unq τ) ~~> ref e
-  | CSwap Γ1 Γ2 a1 a2 τ1 τ2 e1 e2 :
-    Γ1 ⊢ a1 : (Unq τ1) ~~> e1 →
-    Γ2 ⊢ a2 : τ2 ~~> e2 →
-      (Γ1 ∪ Γ2) ⊢ (Swap a1 a2) : (Tensor (Unq τ2) τ1) ~~>
-        let: "l" := e1 in
-        let: "r" := !"l" in
-        let: "_" := "l" <- e2 in ("l", "r")
-where "Γ ⊢ a : τ '~~>' e" := (compile Γ a τ e).
+Section compile.
+  (* I literally just copied this from random STLC notation thing *)
+  Reserved Notation "Γ ⊢ a : τ '~~>' e" (at level 74, a, τ, e at next level).
+
+  Inductive compile : ctx → aexpr → ty → expr → Prop :=
+    | CUnit Γ :
+        Γ ⊢ Unit : One ~~> #()
+    | CVar Γ x τ :
+      Γ !! x = Some τ →
+        Γ ⊢ (Var x) : τ ~~> x
+    | CLam Γ x a τ1 τ2 e :
+      (CtxItem x τ1 :: Γ) ⊢ a : τ2 ~~> e →
+        Γ ⊢ (Lam (BNamed x) a) : (Fun τ1 τ2) ~~> λ: x, e
+    | CApp Γ1 Γ2 a1 a2 τ1 τ2 e1 e2 :
+      Γ1 ⊢ a1 : (Fun τ1 τ2) ~~> e1 →
+      Γ2 ⊢ a2 : τ1 ~~> e2 →
+        (Γ1 ++ Γ2) ⊢ (App a1 a2) : τ2 ~~> e1 e2
+    | CPair Γ1 Γ2 a1 a2 τ1 τ2 e1 e2 :
+      Γ1 ⊢ a1 : τ1 ~~> e1 →
+      Γ2 ⊢ a2 : τ2 ~~> e2 →
+        (Γ1 ++ Γ2) ⊢ (Pair a1 a2) : (Tensor τ1 τ2) ~~> (e1, e2)
+    | CSplit Γ1 Γ2 x1 x2 a1 a2 τ1 τ2 τ e1 e2 :
+      Γ1 ⊢ a1 : (Tensor τ1 τ2) ~~> e1 →
+      (CtxItem x2 τ2 :: CtxItem x1 τ1 :: Γ2) ⊢ a2 : τ ~~> e2 →
+        (Γ1 ++ Γ2) ⊢ (Split (BNamed x1) (BNamed x2) a1 a2) : τ ~~>
+          let: "tmp" := e1 in
+          let: x1 := Fst "tmp" in
+          let: x2 := (Snd "tmp") in e2
+    | CNew Γ a τ e :
+      Γ ⊢ a : τ ~~> e →
+        Γ ⊢ (New a) : (Unq τ) ~~> ref e
+    | CSwap Γ1 Γ2 a1 a2 τ1 τ2 e1 e2 :
+      Γ1 ⊢ a1 : (Unq τ1) ~~> e1 →
+      Γ2 ⊢ a2 : τ2 ~~> e2 →
+        (Γ1 ++ Γ2) ⊢ (Swap a1 a2) : (Tensor (Unq τ2) τ1) ~~>
+          let: "l" := e1 in
+          let: "r" := !"l" in
+          let: "_" := "l" <- e2 in ("l", "r")
+  where "Γ ⊢ a : τ '~~>' e" := (compile Γ a τ e).
+End compile.
+
+(* TODO:
+    update relation to quantify over fresh names *)
