theories/fundamental.v
@@ -1,28 +1,9 @@
-From affi Require Import source.
-From affi Require Import logrel.
+From affi Require Import source logrel helpers.
 From iris.heap_lang Require Import notation lang.
 From iris.proofmode Require Import proofmode tactics.
 From iris.heap_lang Require Import primitive_laws metatheory.
 From iris.heap_lang Require Import proofmode.
 From iris.prelude Require Import options.
-
-
-(* From Semantics notes:
-   The following tactic will be useful for applying bind:
-   [smart_wp_bind e spat v "Hv" He] will bind the subexpression [e],
-   using spat, then will apply the semantic typing assumption [He]
-   for it, introducing the resulting value [v] and interpretation ["Hv"]
-   
-   I added in the spat thing since we have to split hypotheses,
-   but I don't know what `constr` is: I just copied template lol
-   Apparently it means to pass in the argument as a resolved Coq term?
- *)
-Local Tactic Notation "smart_wp_bind"
-    uconstr(e) constr(pat) ident(v) constr(Hv) uconstr(He) :=
-  wp_bind e;
-  iApply (wp_wand with pat); [iApply He; trivial|];
-  simpl; iIntros (v) Hv.
-
 
 Lemma compat_unit Γ :
   Γ ⊨ #() : One.
@@ -40,12 +21,12 @@ Proof.
   iIntros (Hlook γ) "Hg/="; rewrite /expr_interp.
   (* [//] creates a goal for the premise (in this case Γ) with no
      spatial hypotheses, then uses // to call done and solve *)
-  iPoseProof (context_interp_lookup with "[//] Hg") as "[%v [-> Hv]]".
+  iPoseProof (ctx_interp_lookup with "[//] Hg") as "[%v [-> Hv]]".
   iApply wp_value; done. 
 Qed.
 
 Lemma compat_lam Γ (x : string) e τ1 τ2 :
-  (<[x := τ1]> Γ) ⊨ e : τ2 →
+  (CtxItem x τ1 :: Γ) ⊨ e : τ2 →
   Γ ⊨ (λ: x, e) : Fun τ1 τ2.
 Proof.
   iIntros (He γ) "Hg/=". rewrite /expr_interp /fun_interp.
@@ -53,19 +34,20 @@ Proof.
   wp_pure; iModIntro. iIntros (w) "Hvw".
   rewrite /expr_interp. wp_pure.
   iPoseProof (He $! (<[ x := w ]> γ) with "[Hvw Hg]") as "He".
-  - iApply (context_interp_insert with "Hvw Hg").
+  - admit.
+    (* iApply (context_interp_insert with "Hvw Hg"). *)
   (* rewrite -foo is like rewrite <- foo *)
-  - rewrite -subst_map_insert. done.
-Qed.
+  - rewrite -subst_map_insert.
+  Admitted.
 
 Lemma compat_app Γ1 Γ2 e1 e2 τ1 τ2 :
   Γ1 ⊨ e1 : Fun τ1 τ2 →
   Γ2 ⊨ e2 : τ1 →
-  Γ1 ∪ Γ2 ⊨ e1 e2 : τ2.
+  Γ1 ++ Γ2 ⊨ e1 e2 : τ2.
 Proof.
   iIntros (He1 He2 γ) "Hg/="; rewrite /expr_interp.
-  (* OLD: rewrite this_should_hold; iDestruct "Hg" as "[Hg1 Hg2]". *)
-  iDestruct (this_should_hold with "Hg") as "[Hg1 Hg2]".
+  (* OLD: rewrite ctx_interp_split; iDestruct "Hg" as "[Hg1 Hg2]". *)
+  iDestruct (ctx_interp_split with "Hg") as "[Hg1 Hg2]".
   smart_wp_bind (subst_map _ e2) "[Hg2]" v2 "Hv2" He2.
   (* Verbose: 
     wp_bind (subst_map _ e2).
@@ -82,10 +64,10 @@ Qed.
 Lemma compat_pair Γ1 Γ2 e1 e2 τ1 τ2 :
   Γ1 ⊨ e1 : τ1 →
   Γ2 ⊨ e2 : τ2 →
-  Γ1 ∪ Γ2 ⊨ (e1, e2) : (Tensor τ1 τ2).
+  Γ1 ++ Γ2 ⊨ (e1, e2) : (Tensor τ1 τ2).
 Proof.
   iIntros (He1 He2 γ) "Hg/="; rewrite /expr_interp /tensor_interp.
-  iDestruct (this_should_hold with "Hg") as "[Hg1 Hg2]".
+  iDestruct (ctx_interp_split with "Hg") as "[Hg1 Hg2]".
   smart_wp_bind (subst_map _ e2) "[Hg2]" v2 "Hv2" He2.
   smart_wp_bind (subst_map _ e1) "[Hg1]" v1 "Hv1" He1.
   wp_pures; iModIntro. eauto with iFrame.
@@ -93,8 +75,8 @@ Qed.
 
 Lemma compat_split Γ1 Γ2 (x1 x2 : string) e1 e2 τ1 τ2 τ :
   Γ1 ⊨ e1 : Tensor τ1 τ2 →
-  <[x2:=τ2]> (<[x1:=τ1]> Γ2) ⊨ e2 : τ →
-  Γ1 ∪ Γ2 ⊨ (let: "tmp" := e1 in 
+  CtxItem x2 τ2 :: CtxItem x1 τ1 :: Γ2 ⊨ e2 : τ →
+  Γ1 ++ Γ2 ⊨ (let: "tmp" := e1 in 
               let: x1 := Fst "tmp" in 
               let: x2 := Snd "tmp" in e2) : τ.
 Proof.
@@ -112,11 +94,30 @@ Qed.
 Lemma compat_swap Γ1 Γ2 e1 e2 τ1 τ2 :
   Γ1 ⊨ e1 : Unq τ1 →
   Γ2 ⊨ e2 : τ2 →
-  Γ1 ∪ Γ2 ⊨ (let: "l" := e1 in 
+  Γ1 ++ Γ2 ⊨ (let: "l" := e1 in 
               let: "r" := ! "l" in 
               let: "_" := "l" <- e2 in 
                 ("l", "r")) : Tensor (Unq τ2) τ1.
 Proof.
+  iIntros (He1 He2 γ) "Hg/="; rewrite /expr_interp.
+  iDestruct (ctx_interp_split with "Hg") as "[Hg1 Hg2]".
+  smart_wp_bind (subst_map γ e1) "[Hg1]" l "[%loc [%v1 (-> & Hpt & Hv1)]]" He1.
+  rewrite lookup_delete. wp_pures. wp_load. wp_pures.
+  (* Surely there is a better way to do this *)
+  rewrite lookup_delete_ne; auto.
+  rewrite lookup_delete_ne; auto.
+  rewrite lookup_delete. simpl.
+  rewrite -subst_map_insert2; auto.
+  wp_bind (Store _ _). wp_bind (subst_map _ _).
+  (* Problem: we need 
+    𝒢⟦ Γ2 ⟧ (<["l":=#loc]> (<["r":=v1]> γ)) in order to apply
+    He2 to the term.
+    technically this means we can't have l or r appear free in e2
+    the way to enforce that is probably just to require that
+    l and r are not in Γ2, then the proof should fall out
+    I guess I should just update my compilation relation *)
+
+  
   Admitted.
 
 Local Hint Resolve compat_unit compat_var compat_lam compat_app
