theories/helpers.v
@@ -1,0 +1,74 @@
+From affi Require Import source logrel.
+From iris.proofmode Require Import proofmode tactics.
+From iris.heap_lang Require Import proofmode.
+From iris.heap_lang Require Import primitive_laws metatheory.
+From iris.prelude Require Import options.
+
+
+(* From Semantics notes:
+   The following tactic will be useful for applying bind:
+   [smart_wp_bind e spat v "Hv" He] will bind the subexpression [e],
+   using spat, then will apply the semantic typing assumption [He]
+   for it, introducing the resulting value [v] and interpretation ["Hv"]
+   
+   I added in the spat thing since we have to split hypotheses,
+   but I don't know what `constr` is: I just copied template lol
+   Apparently it means to pass in the argument as a resolved Coq term?
+ *)
+Tactic Notation "smart_wp_bind"
+    uconstr(e) constr(pat) ident(v) constr(Hv) uconstr(He) :=
+  wp_bind e;
+  iApply (wp_wand with pat); [iApply He; trivial|];
+  simpl; iIntros (v) Hv.
+
+
+Lemma subst_map_insert2 x1 v1 x2 v2 vs e : x1 ≠ x2 ->
+  subst_map (<[x2:=v2]> (<[x1:=v1]>vs)) e = 
+    subst x1 v1 (subst x2 v2 (subst_map (delete x1 (delete x2 vs)) e)).
+Proof.
+  intros Hneq.
+  (* Room for streamlining *)
+  rewrite subst_subst_ne; auto.
+  rewrite -subst_map_insert.
+  rewrite -delete_insert_ne; auto.
+  rewrite -subst_map_insert; auto.
+Qed.
+
+
+(* Mostly inspired from Semantics notes *)
+Section context_lemmas.
+  Lemma ctx_lookup_contains (Γ : ctx) x τ : 
+    Γ !! x = Some τ → CtxItem x τ ∈ Γ.
+  Proof.
+    (* By induction on Γ, using ctx_lookup definition
+        Admitted for now because this is clearly true but annoying *)
+    Admitted.
+
+  Lemma ctx_interp_split Γ1 Γ2 γ :
+    𝒢⟦ Γ1 ++ Γ2 ⟧ γ ⊣⊢ 𝒢⟦ Γ1 ⟧ γ ∗ 𝒢⟦ Γ2 ⟧ γ.
+  Proof.
+    iApply big_sepL_app.
+  Qed.
+
+  Lemma ctx_interp_lookup Γ γ τ x :
+    ⌜Γ !! x = Some τ⌝ -∗
+    𝒢⟦ Γ ⟧ γ -∗
+    ∃ v, ⌜γ !! x = Some v⌝ ∗ 𝒱⟦ τ ⟧ v.
+  Proof.
+    iIntros (Hlook) "Hγ".
+    apply ctx_lookup_contains in Hlook.
+    iPoseProof (big_sepL_elem_of _ Γ _ with "Hγ") as "HΦ"; done.
+  Qed.
+
+  (* TODO: come back and prove this, in the case where x is not in Γ
+  (Also prove the thing from the Swap compat lemma, where we add to γ only)
+
+  Lemma ctx_interp_insert Γ γ τ v x :
+    𝒱⟦ τ ⟧ v -∗
+    𝒢⟦ Γ ⟧ γ -∗
+    𝒢⟦ (<[ x := τ ]> Γ) ⟧ (<[ x := v ]> γ).
+  Proof.
+    iIntros "Hv Hγ". iApply (big_sepM2_insert_2 with "[Hv] [Hγ]"); done.
+  Qed.
+  *)
+End context_lemmas.
